examples/dynamic_isolation/External.v
@@ -1,0 +1,46 @@
+Require Import Koika.Frontend.
+Require Import Koika.Std.
+
+Require Import DynamicIsolation.Interfaces.
+
+Module External <: External_sig.
+  Import Common.
+  Inductive memory := imem | dmem.
+
+  Inductive ext_fn_t' :=
+  | ext_mem (m: memory)
+  | ext_uart_read
+  | ext_uart_write
+  | ext_led.
+
+  Definition ext_fn_t := ext_fn_t'.
+  Definition led_input := maybe (bits_t 1).
+  Definition uart_input := maybe (bits_t 8).
+  Definition uart_output := maybe (bits_t 8).
+
+  Definition Sigma (fn: ext_fn_t) :=
+    match fn with
+    | ext_mem _ => {$ struct_t mem_input ~> struct_t mem_output $}
+    | ext_uart_read => {$ bits_t 1 ~> uart_output $}
+    | ext_uart_write => {$ uart_input ~> bits_t 1 $}
+    | ext_led => {$ led_input ~> bits_t 1 $}
+    end.
+
+  Definition sigma (fn: ext_fn_t) : Sig_denote (Sigma fn). Admitted.
+
+  Definition ext_fn_specs (fn: ext_fn_t) :=
+    match fn with
+    | ext_mem imem => {| ef_name := "ext_mem_imem"; ef_internal := false |}
+    | ext_mem dmem => {| ef_name := "ext_mem_dmem"; ef_internal := false |}
+    | ext_uart_write => {| ef_name := "ext_uart_write"; ef_internal := false |}
+    | ext_uart_read => {| ef_name := "ext_uart_read"; ef_internal := false |}
+    | ext_led => {| ef_name := "ext_led"; ef_internal := false |}
+    end.
+
+  Instance Show_ext_fn_t : Show ext_fn_t := _.
+
+End External.
+
+Module EnclaveParams <: EnclaveParameters.
+
+End EnclaveParams.
