examples/dynamic_isolation/Memory.v
@@ -1,0 +1,155 @@
+Require Import Koika.Frontend.
+Require Import Coq.Lists.List.
+
+Require Import Koika.Std.
+Require Import DynamicIsolation.RVEncoding.
+Require Import DynamicIsolation.Scoreboard.
+Require Import DynamicIsolation.Multiplier.
+
+Require Import DynamicIsolation.External.
+Require Import DynamicIsolation.Tactics.
+Require Import DynamicIsolation.Interfaces.
+
+Module Memory <: Memory_sig External.
+  Import Common.
+
+  Inductive internal_reg_t' : Type := .
+  Definition internal_reg_t := internal_reg_t'.
+  Definition R_internal (idx: internal_reg_t) : type :=
+    match idx with end.
+
+  Definition r_internal (idx: internal_reg_t) : R_internal idx :=
+    match idx with end.
+
+  Inductive reg_t :=
+  | toIMem0 (state: MemReq.reg_t)
+  | toIMem1 (state: MemReq.reg_t)
+  | toDMem0 (state: MemReq.reg_t)
+  | toDMem1 (state: MemReq.reg_t)
+  | fromIMem0 (state: MemResp.reg_t)
+  | fromIMem1 (state: MemResp.reg_t)
+  | fromDMem0 (state: MemResp.reg_t)
+  | fromDMem1 (state: MemResp.reg_t)
+  | internal (r: internal_reg_t)
+  .
+
+  Definition R (idx: reg_t) :=
+    match idx with
+    | toIMem0 st => MemReq.R st
+    | toIMem1 st => MemReq.R st
+    | toDMem0 st => MemReq.R st
+    | toDMem1 st => MemReq.R st
+    | fromIMem0 st => MemResp.R st
+    | fromIMem1 st => MemResp.R st
+    | fromDMem0 st => MemResp.R st
+    | fromDMem1 st => MemResp.R st
+    | internal st => R_internal st
+    end.
+
+  Definition ext_fn_t := External.ext_fn_t.
+  Definition Sigma := External.Sigma.
+  Definition rule := rule R Sigma.
+  Definition sigma := External.sigma.
+
+
+  Definition MMIO_UART_ADDRESS := Ob~0~1~0~0~0~0~0~0~0~0~0~0~0~0~0~0~0~0~0~0~0~0~0~0~0~0~0~0~0~0~0~0.
+  Definition MMIO_LED_ADDRESS  := Ob~0~1~0~0~0~0~0~0~0~0~0~0~0~0~0~0~0~0~0~0~0~0~0~0~0~0~0~0~0~1~0~0.
+
+  Import External.
+
+  Definition memoryBus (m: memory) : UInternalFunction reg_t ext_fn_t :=
+    {{ fun memoryBus (get_ready: bits_t 1) (put_valid: bits_t 1) (put_request: struct_t mem_req) : struct_t mem_output =>
+         `match m with
+          | imem => {{ extcall (ext_mem m) (struct mem_input {|
+                        get_ready := get_ready;
+                        put_valid := put_valid;
+                        put_request := put_request |}) }}
+          | dmem => {{ let addr := get(put_request, addr) in
+                      let byte_en := get(put_request, byte_en) in
+                      let is_write := byte_en == Ob~1~1~1~1 in
+
+                      let is_uart := addr == #MMIO_UART_ADDRESS in
+                      let is_uart_read := is_uart && !is_write in
+                      let is_uart_write := is_uart && is_write in
+
+                      let is_led := addr == #MMIO_LED_ADDRESS in
+                      let is_led_write := is_led && is_write in
+
+                      let is_mem := !is_uart && !is_led in
+
+                      if is_uart_write then
+                        let char := get(put_request, data)[|5`d0| :+ 8] in
+                        let may_run := get_ready && put_valid && is_uart_write in
+                        let ready := extcall ext_uart_write (struct (Maybe (bits_t 8)) {|
+                          valid := may_run; data := char |}) in
+                        struct mem_output {| get_valid := may_run && ready;
+                                             put_ready := may_run && ready;
+                                             get_response := struct mem_resp {|
+                                               byte_en := byte_en; addr := addr;
+                                               data := |32`d0| |} |}
+
+                      else if is_uart_read then
+                        let may_run := get_ready && put_valid && is_uart_read in
+                        let opt_char := extcall ext_uart_read (may_run) in
+                        let ready := get(opt_char, valid) in
+                        struct mem_output {| get_valid := may_run && ready;
+                                             put_ready := may_run && ready;
+                                             get_response := struct mem_resp {|
+                                               byte_en := byte_en; addr := addr;
+                                               data := zeroExtend(get(opt_char, data), 32) |} |}
+
+                      else if is_led then
+                        let on := get(put_request, data)[|5`d0|] in
+                        let may_run := get_ready && put_valid && is_led_write in
+                        let current := extcall ext_led (struct (Maybe (bits_t 1)) {|
+                          valid := may_run; data := on |}) in
+                        let ready := Ob~1 in
+                        struct mem_output {| get_valid := may_run && ready;
+                                             put_ready := may_run && ready;
+                                             get_response := struct mem_resp {|
+                                               byte_en := byte_en; addr := addr;
+                                               data := zeroExtend(current, 32) |} |}
+
+                      else
+                        extcall (ext_mem m) (struct mem_input {|
+                          get_ready := get_ready && is_mem;
+                          put_valid := put_valid && is_mem;
+                          put_request := put_request |})
+                   }}
+          end` }}.
+
+  Definition mem (m: memory) : uaction reg_t ext_fn_t :=
+    let fromMem := match m with imem => fromIMem0 | dmem => fromDMem0 end in
+    let toMem := match m with imem => toIMem0 | dmem => toDMem0 end in
+    {{
+        let get_ready := fromMem.(MemResp.can_enq)() in
+        let put_request_opt := toMem.(MemReq.peek)() in
+        let put_request := get(put_request_opt, data) in
+        let put_valid := get(put_request_opt, valid) in
+        let mem_out := {memoryBus m}(get_ready, put_valid, put_request) in
+        (when (get_ready && get(mem_out, get_valid)) do fromMem.(MemResp.enq)(get(mem_out, get_response)));
+        (when (put_valid && get(mem_out, put_ready)) do ignore(toMem.(MemReq.deq)()))
+    }}.
+
+  Definition tc_imem := tc_rule R Sigma (mem imem) <: rule.
+  Definition tc_dmem := tc_rule R Sigma (mem dmem) <: rule.
+
+  Inductive rule_name_t' :=
+  | Imem
+  | Dmem
+  .
+
+  Definition rule_name_t := rule_name_t'.
+
+  Definition rules (rl: rule_name_t) : rule :=
+    match rl with
+    | Imem           => tc_imem
+    | Dmem           => tc_dmem
+    end.
+
+  Definition schedule : scheduler :=
+    Imem |> Dmem |> done.
+
+  Instance FiniteType_internal_reg_t : FiniteType internal_reg_t := _.
+  Instance FiniteType_reg_t : FiniteType reg_t := _.
+End Memory.
