examples/dynamic_isolation/TrivialCore.v
@@ -1,0 +1,68 @@
+Require Import Koika.Frontend.
+Require Import Koika.Std.
+
+Require Import DynamicIsolation.External.
+Require Import DynamicIsolation.Interfaces.
+
+
+Module EmptyCore (External: External_sig) (Params: EnclaveParameters) (CoreParams: CoreParameters) 
+                 <: Core_sig External Params CoreParams.
+  Import Common.
+
+  Inductive internal_reg_t' : Type := .
+  Definition internal_reg_t := internal_reg_t'.
+  Definition R_internal (idx: internal_reg_t) : type :=
+    match idx with end.
+
+  Definition r_internal (idx: internal_reg_t) : R_internal idx :=
+    match idx with end.
+
+  Inductive reg_t :=
+  | core_id
+  | pc
+  | toIMem (state: MemReq.reg_t)
+  | toDMem (state: MemReq.reg_t)
+  | fromIMem (state: MemResp.reg_t)
+  | fromDMem (state: MemResp.reg_t)
+  | internal (r: internal_reg_t)
+  .
+
+  Definition R (idx: reg_t) : type :=
+   match idx with
+   | core_id => bits_t 1
+   | pc => addr_t
+   | toIMem r => MemReq.R r
+   | toDMem r => MemReq.R r
+   | fromIMem  r => MemResp.R r
+   | fromDMem  r => MemResp.R r
+   | internal r => R_internal r
+   end.
+
+  Definition r idx : R idx :=
+    match idx with
+    | core_id => CoreParams.core_id
+    | pc => Bits.zero
+    | toIMem s => MemReq.r s
+    | fromIMem s => MemResp.r s
+    | toDMem s => MemReq.r s
+    | fromDMem s => MemResp.r s
+    | internal s => r_internal s
+    end.
+
+  Definition ext_fn_t := External.ext_fn_t.
+  Definition Sigma := External.Sigma.
+  Definition rule := rule R Sigma.
+  Definition sigma := External.sigma.
+
+  Inductive rule_name_t' : Type := .
+  Definition rule_name_t := rule_name_t'.
+
+  Definition rules (rl: rule_name_t) : rule :=
+    match rl with end.
+
+  Definition schedule : Syntax.scheduler pos_t rule_name_t := done.
+
+  Instance FiniteType_internal_reg_t : FiniteType internal_reg_t := _.
+  Instance FiniteType_reg_t : FiniteType reg_t := _.
+
+End EmptyCore.
