examples/dynamic_isolation/rv32.v
@@ -1,31 +1,77 @@
-(*! Definition of a pipelined schedule !*)
 Require Import Koika.Frontend.
+
+Require Import DynamicIsolation.External.
+Require Import DynamicIsolation.Interfaces.
+Require Import DynamicIsolation.Memory.
 Require Import DynamicIsolation.RVCore.
+Require Import DynamicIsolation.TrivialCore.
 
-Definition rv_schedule : scheduler :=
-  Writeback |> Execute |> StepMultiplier |> Decode |> WaitImem |> Fetch |> Imem |> Dmem |> Tick |> done.
+Module Params0 <: CoreParameters.
+  Definition core_id := Ob~0.
+End Params0.
 
-Module Package (C: Core).
-  Import C.
-  Existing Instance Show_reg_t.
-  Existing Instance Show_ext_fn_t.
-  Existing Instance FiniteType_reg_t.
+Module Params1 <: CoreParameters.
+  Definition core_id := Ob~1.
+End Params1.
+
+Module Core0_rv32i := RV32I EnclaveParams Params0.
+Module Core0_rv32e := RV32E EnclaveParams Params0.
+Module Core1 := EmptyCore External EnclaveParams Params1.
+Module Mem := Memory.
+
+(* TODO: modularize *)
+
+Module Machine_rv32i := Machine External EnclaveParams Params0 Params1
+                        Core0_rv32i Core1 Mem.
+Module Machine_rv32e := Machine External EnclaveParams Params0 Params1
+                        Core0_rv32e Core1 Mem.
+
+Module Package_rv32i.
+  Include Machine_rv32i.
+  Definition external (rl: rule_name_t) := false.
 
   Definition circuits :=
-    compile_scheduler rv_rules rv_external rv_schedule.
+    compile_scheduler rules external schedule.
 
   Definition koika_package :=
     {| koika_reg_types := R;
        koika_reg_init := r;
        koika_ext_fn_types := Sigma;
-       koika_rules := rv_rules;
-       koika_rule_external := rv_external;
-       koika_scheduler := rv_schedule;
+       koika_rules := rules;
+       koika_rule_external := external;
+       koika_scheduler := schedule;
        koika_module_name := "rv32" |}.
 
   Definition package :=
     {| ip_koika := koika_package;
        ip_sim := {| sp_ext_fn_names fn := show fn;
                    sp_extfuns := None |};
-       ip_verilog := {| vp_ext_fn_specs := rv_ext_fn_specs |} |}.
-End Package.
+       ip_verilog := {| vp_ext_fn_specs := ext_fn_specs |} |}.
+
+End Package_rv32i.
+
+Module Package_rv32e.
+  Include Machine_rv32e.
+  Instance Show_reg_t : Show reg_t := _.
+
+  Definition external (rl: rule_name_t) := false.
+
+  Definition circuits :=
+    compile_scheduler rules external schedule.
+
+  Definition koika_package :=
+    {| koika_reg_types := R;
+       koika_reg_init := r;
+       koika_ext_fn_types := Sigma;
+       koika_rules := rules;
+       koika_rule_external := external;
+       koika_scheduler := schedule;
+       koika_module_name := "rv32" |}.
+
+  Definition package :=
+    {| ip_koika := koika_package;
+       ip_sim := {| sp_ext_fn_names fn := show fn;
+                   sp_extfuns := None |};
+       ip_verilog := {| vp_ext_fn_specs := ext_fn_specs |} |}.
+
+End Package_rv32e.
