examples/dynamic_isolation/rv32e.v
@@ -1,5 +1,5 @@
 (*! Pipelined instantiation of an RV32E core !*)
-Require Import DynamicIsolation.RVCore DynamicIsolation.rv32.
-Module RV32EPackage := Package RV32E.
+Require Import DynamicIsolation.rv32.
+Module RV32EPackage := Package_rv32e.
 Definition prog := Interop.Backends.register RV32EPackage.package.
 Extraction "rv32e.ml" prog.
