examples/dynamic_isolation/rv32i.v
@@ -1,5 +1,5 @@
 (*! Pipelined instantiation of an RV32I core !*)
-Require Import DynamicIsolation.RVCore DynamicIsolation.rv32.
-Module RV32IPackage := Package RV32I.
+Require Import DynamicIsolation.rv32.
+Module RV32IPackage := Package_rv32i.
 Definition prog := Interop.Backends.register RV32IPackage.package.
 Extraction "rv32i.ml" prog.
